WIP

code/ecdsa/Hacl.Impl.EC.ScalarMult.Radix.fst
@@ -30,9 +30,10 @@ open Hacl.Spec.EC.ScalarMult.Radix
 
 #set-options "--z3rlimit 200 --max_ifuel 0 --max_fuel 0 "
 
-
 inline_for_extraction noextract
-val getPointDoubleNTimes: #c: curve -> p: point c -> tempBuffer: lbuffer uint64 (size 17 *! getCoordinateLenU64 c) ->
+val getPointDoubleNTimes: #c: curve 
+  -> p: point c 
+  -> tempBuffer: lbuffer uint64 (size 17 *! getCoordinateLenU64 c) ->
   Stack unit
   (requires fun h -> live h p /\ live h tempBuffer /\ disjoint p tempBuffer /\ point_eval c h p)
   (ensures fun h0 _ h1 -> modifies (loc p |+| loc tempBuffer) h0 h1 /\ point_eval c h1 p /\
@@ -51,7 +52,8 @@ let getPointDoubleNTimes #c p tempBuffer =
     unfold_repeat 4 (_point_double #c) (fromDomainPoint #c #DH (point_as_nat c h0 p)) (v i))
 
 
-val curve_compatibility_with_translation_lemma_1: #c: curve -> p: Spec.ECC.point #c #Jacobian 
+val curve_compatibility_with_translation_lemma_1: #c: curve 
+  -> p: Spec.ECC.point #c #Jacobian 
   -> p1: Spec.ECC.point #c #Jacobian
   -> q: Spec.ECC.point #c #Jacobian -> 
   Lemma (pointEqual p p1 <==> pointEqual (pointAdd #c q p) (pointAdd #c q p1))
@@ -62,17 +64,19 @@ let curve_compatibility_with_translation_lemma_1 #c p p1 q =
   curve_commutativity_lemma p1 q
 
 
-val point_mult_mult0: #c: curve -> a: nat -> k: nat
+val lemma_point_mult_addition_of_coefficients: #c: curve 
+  -> a: nat 
+  -> k: nat
   -> p: Spec.ECC.point #c #Jacobian ->
   Lemma (pointEqual (pointAdd (point_mult a p) (point_mult k p)) (point_mult (k + a) p))
 
-let rec point_mult_mult0 #c a k p = 
+let rec lemma_point_mult_addition_of_coefficients #c a k p = 
   match a with
   | 0 -> 
     point_mult_0 p 0;
     curve_point_at_infinity_property (point_mult k p)
   | _ -> 
-    point_mult_mult0 #c (a - 1) k p;
+    lemma_point_mult_addition_of_coefficients #c (a - 1) k p;
     let pa = point_mult a p in  
     let pa1 = point_mult (a - 1) p in  
     let kp = point_mult k p in 
@@ -86,22 +90,24 @@ let rec point_mult_mult0 #c a k p =
     curve_compatibility_with_translation_lemma (pointAdd #c p pa1) pa kp
 
 
-val point_mult_mult1: a: nat -> b: nat -> Lemma (a * (b - 1) + a == a * b)
+val lemma_nat_distribitivity: a: nat -> b: nat -> Lemma (a * (b - 1) + a == a * b)
 
-let point_mult_mult1 a b = ()
+let lemma_nat_distribitivity a b = ()
 
 
-val point_mult_mult: #c: curve -> a: nat -> b: nat 
-  -> p: Spec.ECC.point #c #Jacobian -> Lemma (
-  pointEqual (point_mult b (point_mult a p)) (point_mult (a * b) p))
+val lemma_point_mult_associativity: #c: curve 
+  -> a: nat 
+  -> b: nat 
+  -> p: Spec.ECC.point #c #Jacobian -> 
+  Lemma (pointEqual (point_mult b (point_mult a p)) (point_mult (a * b) p))
 
-let rec point_mult_mult #c a b p = 
+let rec lemma_point_mult_associativity #c a b p = 
   match b with 
   |0 -> 
     point_mult_0 p 0;
     point_mult_0 (point_mult a p) 0
   |_ ->
-    point_mult_mult #c a (b - 1) p;
+    lemma_point_mult_associativity #c a (b - 1) p;
     assert(pointEqual (point_mult (b - 1) (point_mult a p)) (point_mult (a * (b - 1)) p));
 
     let pa = point_mult a p in 
@@ -111,52 +117,42 @@ let rec point_mult_mult #c a b p =
 
     point_mult_ext #c (b - 1) pa; 
 
-    point_mult_mult0 a (a * (b - 1)) p;
-    point_mult_mult1 a b;
+    lemma_point_mult_addition_of_coefficients a (a * (b - 1)) p;
+    lemma_nat_distribitivity a b;
     assert(pointEqual (pointAdd (point_mult a p) (point_mult (a * (b - 1)) p)) (point_mult (a * b) p));
-
 
     curve_compatibility_with_translation_lemma_1 (point_mult (b - 1) pa) (point_mult (a * (b - 1)) p) pa;
     curve_compatibility_with_translation_lemma (pointAdd #c pa (point_mult (b - 1) pa)) (point_mult b pa) (pointAdd pa (point_mult (a * (b - 1)) p));
     curve_compatibility_with_translation_lemma (pointAdd #c pa (point_mult (a * (b - 1)) p)) (point_mult (a * b) p) (point_mult b pa)
 
 
-val not_equal_precomputed0: #c: curve 
-    -> a: nat
-    -> p0: Spec.ECC.point #c #Jacobian 
-    -> p1: Spec.ECC.point #c #Jacobian {pointEqual p0 p1} -> 
-    Lemma (pointEqual (point_mult a p0) (point_mult a p1))
+val lemma_point_mult_equal_points: #c: curve 
+  -> p0: Spec.ECC.point #c 
+  -> p1: Spec.ECC.point #c {pointEqual p0 p1} 
+  -> i: nat -> 
+  Lemma (pointEqual (point_mult i p0) (point_mult i p1))
 
-let rec not_equal_precomputed0 #c a p0 p1 = 
-  match a with 
-  |0 ->
-    point_mult_0 #c p0 0; 
-    point_mult_0 #c p1 0
+let rec lemma_point_mult_equal_points #c p0 p1 i = 
+  match i with 
+  |0 -> point_mult_0 p0 0; point_mult_0 p1 0
   |_ -> 
-    not_equal_precomputed0 #c (a - 1) p0 p1;
-    point_mult_ext (a - 1) p0;
-    point_mult_ext (a - 1) p1;
-
-    assert(pointEqual (point_mult (a - 1) p0) (point_mult (a - 1) p1));
-    assert(pointEqual (pointAdd p0 (point_mult (a - 1) p0)) (point_mult a p0));
-    assert(pointEqual (pointAdd p1 (point_mult (a - 1) p1)) (point_mult a p1));
-
-    curve_compatibility_with_translation_lemma_1 (point_mult (a - 1) p0) (point_mult (a - 1) p1) p0;
-    curve_compatibility_with_translation_lemma_1 (pointAdd p0 (point_mult (a - 1) p0)) (point_mult a p0) (pointAdd p0 (point_mult (a - 1) p1));
-    curve_compatibility_with_translation_lemma p0 p1 (point_mult (a - 1) p1);
-    curve_compatibility_with_translation_lemma_1 (pointAdd p1 (point_mult (a - 1) p1)) (point_mult a p1) (point_mult a p0);
-    assert(pointEqual (point_mult a p0) (pointAdd p1 (point_mult (a - 1) p1)))
+    lemma_point_mult_equal_points #c p0 p1 (i - 1);
+    point_mult_ext (i - 1) p0;
+    point_mult_ext (i - 1) p1; 
+    curve_compatibility_with_translation_lemma p0 p1 (point_mult (i - 1) p0);
+    curve_compatibility_with_translation_lemma_1  (point_mult (i - 1) p0) (point_mult (i - 1) p1) p1
 
 
-val point_mult_of_point_infinity: #c: curve -> p: Spec.ECC.point #c {isPointAtInfinity #c p} 
+val lemma_point_mult_of_point_infinity: #c: curve 
+  -> p: Spec.ECC.point #c {isPointAtInfinity #c p} 
   -> a: nat ->
   Lemma (isPointAtInfinity (point_mult a p))
 
-let rec point_mult_of_point_infinity #c p a = 
+let rec lemma_point_mult_of_point_infinity #c p a = 
   match a with 
   |0 -> point_mult_0 p 0 
   |_ -> 
-    point_mult_of_point_infinity #c p (a - 1);
+    lemma_point_mult_of_point_infinity #c p (a - 1);
     curve_point_at_infinity_property (point_mult (a - 1) p);
     point_mult_ext (a - 1) p
 
@@ -164,8 +160,8 @@ let rec point_mult_of_point_infinity #c p a =
 val not_equal_precomputed1: #c: curve 
   -> a: nat {a <= 16} 
   -> b: nat {b < getOrder #c}
-  -> p0: Spec.ECC.point #c #Jacobian
-  -> Lemma (
+  -> p0: Spec.ECC.point #c #Jacobian -> 
+  Lemma (
     let pa = point_mult #c a p0 in 
     let pb = point_mult #c b p0 in 
     ~ (pointEqual pa pb) \/ (isPointAtInfinity #c #Jacobian pa /\ isPointAtInfinity #c #Jacobian pb))
@@ -175,8 +171,8 @@ let not_equal_precomputed1 #c a b p0 =
   let pb = point_mult #c b p0 in  
 
   if (isPointAtInfinity #c p0) then begin
-     point_mult_of_point_infinity p0 a;
-     point_mult_of_point_infinity p0 b
+     lemma_point_mult_of_point_infinity p0 a;
+     lemma_point_mult_of_point_infinity p0 b
     end
   else 
     if a = 0 || b = 0 then 
@@ -187,11 +183,11 @@ let not_equal_precomputed1 #c a b p0 =
 	let inv_pb = point_mult #c (getOrder #c - b) p0 in 
 	curve_compatibility_with_translation_lemma pa pb inv_pb;
 	
-	point_mult_mult0 #c b (getOrder #c - b) p0;
+	lemma_point_mult_addition_of_coefficients #c b (getOrder #c - b) p0;
 	point_mult_0 p0 (getOrder #c); 
 	assert(isPointAtInfinity (pointAdd pb inv_pb));
 
-	point_mult_mult0 #c a (getOrder #c - b) p0;
+	lemma_point_mult_addition_of_coefficients #c a (getOrder #c - b) p0;
 	assert(pointEqual (pointAdd pa inv_pb) (point_mult (a - b + getOrder #c) p0));
 
 	curve_order_is_the_smallest p0;  
@@ -205,16 +201,17 @@ val not_equal_precomputed: #c: curve
   -> z: nat
   -> p: Spec.ECC.point #c #Jacobian
   -> p0: Spec.ECC.point #c #Jacobian 
-  -> si: nat {si <= 16} -> Lemma
-    (requires ((z <= getOrder #c / 16) /\ pointEqual p (point_mult #c z p0)))
-    (ensures (
-      let p_16 = Spec.ECC.Radix.getPointDoubleNTimes #c p 4 in 
-      ~ (pointEqual #c p_16 (point_mult #c si p0)) \/ (
-      isPointAtInfinity #c #Jacobian p_16 /\ isPointAtInfinity #c #Jacobian (point_mult #c si p0))))
+  -> si: nat {si <= 16} -> 
+  Lemma
+  (requires ((z <= getOrder #c / 16) /\ pointEqual p (point_mult #c z p0)))
+  (ensures (
+    let p_16 = Spec.ECC.Radix.getPointDoubleNTimes #c p 4 in 
+    ~ (pointEqual #c p_16 (point_mult #c si p0)) \/ (
+    isPointAtInfinity #c #Jacobian p_16 /\ isPointAtInfinity #c #Jacobian (point_mult #c si p0))))
 
 let not_equal_precomputed #c z p p0 si = 
-  point_mult_mult #c z 16 p0;
-  not_equal_precomputed0 16 (point_mult z p0) p;
+  lemma_point_mult_associativity #c z 16 p0;
+  lemma_point_mult_equal_points (point_mult z p0) p 16;
   not_equal_precomputed1 #c si (16 * z) p0
 
 
@@ -246,7 +243,8 @@ val not_equal_precomputed2: #c: curve
   -> p0: Spec.ECC.point #c #Jacobian
   -> p: Spec.ECC.point #c #Jacobian
        { exists (z: nat {z <= getOrder #c / 16}). pointEqual p (point_mult #c z p0)}
-  -> si: nat {si <= 16} -> Lemma (
+  -> si: nat {si <= 16} -> 
+  Lemma (
     let p_16 = Spec.ECC.Radix.getPointDoubleNTimes #c p 4 in 
     ~ (pointEqual #c p_16 (point_mult #c si p0)) \/ (
     isPointAtInfinity #c #Jacobian p_16 /\ isPointAtInfinity #c #Jacobian (point_mult #c si p0)))
@@ -256,10 +254,11 @@ let not_equal_precomputed2 #c p0 p si =
   not_equal_precomputed #c z p p0 si
   
   
-val radix_step_precomputed0: #c: curve -> p: Spec.ECC.point #c #Jacobian {isPointAtInfinity #c p} -> 
+val lemma_point_at_infinity_after_point_double: #c: curve 
+  -> p: Spec.ECC.point #c #Jacobian {isPointAtInfinity #c p} -> 
   Lemma (isPointAtInfinity #c (_point_double p))
 
-let radix_step_precomputed0 #c p = 
+let lemma_point_at_infinity_after_point_double #c p = 
   let pd = _point_double p in 
   
   let prime = getPrime c in 
@@ -286,9 +285,9 @@ val radix_step_precomputed: #c: curve -> #buf_type: buftype
   Stack unit
   (requires fun h -> 
     live h p /\ live h tempBuffer /\ live h scalar /\ point_eval c h p /\ (
-    let fromDomainP_h0 = fromDomainPoint #c #DH (point_as_nat c h p) in 
+    let fromDomainP = fromDomainPoint #c #DH (point_as_nat c h p) in 
     exists (z: nat {z <= getOrder #c / 16}). 
-      pointEqual fromDomainP_h0 (point_mult #c z (basePoint #c)) /\
+      pointEqual fromDomainP (point_mult #c z (basePoint #c)) /\
     LowStar.Monotonic.Buffer.all_disjoint [loc p; loc tempBuffer; loc scalar]))
   (ensures fun h0 _ h1 -> modifies (loc p |+| loc tempBuffer) h0 h1 /\ point_eval c h1 p /\ (
     let fromDomainP_h0 = fromDomainPoint #c #DH (point_as_nat c h0 p) in 
@@ -309,8 +308,8 @@ let radix_step_precomputed #c p tempBuffer scalar i =
     let h3 = ST.get() in
     pop_frame();
 
-    let k = as_seq h0 scalar in 
-    let scalar = scalar_as_nat k in 
+
+    let scalar = scalar_as_nat (as_seq h0 scalar) in 
     let si = Math.Lib.arithmetic_shift_right scalar (v (getScalarLen c) - ((v i - 1) + 2) * 4) % pow2 4 in  
     let pRadixed = Spec.ECC.Radix.getPointDoubleNTimes #c (fromDomainPoint #c #DH (point_as_nat c h0 p)) 4 in
     let pointPrecomputed = Spec.ECC.Radix.getPrecomputedPoint #c #Affine (basePoint #c) si in 
@@ -320,7 +319,7 @@ let radix_step_precomputed #c p tempBuffer scalar i =
     not_equal_precomputed2 #c (basePoint #c) (fromDomainPoint #c #DH (point_as_nat c h0 p)) si;
 
     if (isPointAtInfinity #c #Jacobian pRadixed && isPointAtInfinity #c #Jacobian pointPrecomputed) then 
-	radix_step_precomputed0 #c pRadixed
+	lemma_point_at_infinity_after_point_double #c pRadixed
     else
       begin 
 	curve_compatibility_with_translation_lemma_1 (fromDomainPoint #c #DH (toJacobianCoordinates #c (point_affine_as_nat c h1 pointToAdd))) pointPrecomputed pRadixed;
@@ -329,7 +328,8 @@ let radix_step_precomputed #c p tempBuffer scalar i =
 
 
 inline_for_extraction noextract
-val radix_precomputed_upload_point: #c: curve -> #buf_type: buftype -> p: point c
+val radix_precomputed_upload_point: #c: curve -> #buf_type: buftype 
+  -> p: point c
   -> scalar: lbuffer_t buf_type uint8 (getScalarLenBytes c) ->  
   Stack unit 
   (requires fun h -> live h p /\ live h scalar)
@@ -342,13 +342,11 @@ let radix_precomputed_upload_point #c p scalar =
   let pXpY = sub p (size 0) (size 2 *! getCoordinateLenU64 c) in 
   getPointPrecomputedMixed scalar (size 0) pXpY; 
     let h1 = ST.get() in 
-
   let pZ = sub p (size 2 *! getCoordinateLenU64 c) (getCoordinateLenU64 c) in 
   Hacl.Impl.EC.LowLevel.uploadOneImpl pZ;
     let h2 = ST.get() in 
     
   let pX, pY = point_affine_as_nat c h1 pXpY in 
-
   if isPointAtInfinity #c #Affine (pX, pY) then 
     begin
       Hacl.Spec.MontgomeryMultiplication.lemma_pointAtInfInDomain #c 0 0 0;
@@ -362,8 +360,39 @@ let radix_precomputed_upload_point #c p scalar =
     (point_mult #c (Math.Lib.arithmetic_shift_right (scalar_as_nat (as_seq h0 scalar)) (v (getScalarLen c) - 4) % pow2 4) (basePoint #c)))
 
 
+val lemma_scalar_less_than_order_: #c: curve 
+  -> scalar: nat {scalar < getOrder #c} 
+  -> i: nat {i > 0 /\ i < v ((size 2 *! getScalarLenBytes c))} -> 
+  Lemma (scalar / pow2 4 <= (getOrder #c) / pow2 4)
+
+let lemma_scalar_less_than_order_ #c scalar i = 
+  let o = getOrder #c in 
+  assert(scalar <= o - 1);
+  Math.Lemmas.lemma_div_le scalar (o - 1) (pow2 4);
+  assert(scalar / (pow2 4) <= (o - 1) / (pow2 4));
+  assert(o - 1 < o);
+  Math.Lemmas.lemma_div_le (o - 1) o (pow2 4);
+  assert((o - 1) / pow2 4 <= o / pow2 4);
+  assert(scalar / pow2 4 <= o / pow2 4)
+
+
+val lemma_scalar_less_than_order: #c: curve 
+  -> scalar: nat {scalar < getOrder #c} 
+  -> i: nat {i > 0 /\ i < v ((size 2 *! getScalarLenBytes c))} -> 
+  Lemma (scalar / pow2 ((v (getScalarLen c) - i * 4)) <= (getOrder #c) / pow2 4)
+
+let lemma_scalar_less_than_order #c scalar i = 
+  lemma_scalar_less_than_order_ #c scalar i;
+  assert(v (getScalarLen c) - 4 * i >= 4);
+  Math.Lemmas.pow2_le_compat (v (getScalarLen c) - 4 * i) 4;
+  assert(pow2 (v (getScalarLen c) - 4 * i) >= pow2 4);
+  assert(1 / (pow2 (v (getScalarLen c) - 4 * i)) <= 1 / pow2 4);
+  Math.Lemmas.lemma_mult_le_left scalar (1 / (pow2 (v (getScalarLen c) - 4 * i))) (1 / pow2 4);
+  assert(scalar * (1 / (pow2 (v (getScalarLen c) - 4 * i))) <= scalar / pow2 4)
+
+
 inline_for_extraction noextract
-val montgomery_ladder_2_precomputed: #c: curve -> #buf_type: buftype 
+val secret_to_public_radix: #c: curve -> #buf_type: buftype 
   -> p: point c  
   -> scalar: lbuffer_t buf_type uint8 (getScalarLenBytes c) 
   -> tempBuffer: lbuffer uint64 (size 17 *! getCoordinateLenU64 c)  -> 
@@ -376,34 +405,7 @@ val montgomery_ladder_2_precomputed: #c: curve -> #buf_type: buftype
     pointEqual p_n (point_mult #c (scalar_as_nat (as_seq h0 scalar)) (basePoint #c))))
 
 
-val lemma_test_2: #c: curve ->  scalar: nat {scalar < getOrder #c} 
-  -> i: nat {i > 0 /\ i < v ((size 2 *! getScalarLenBytes c))} -> Lemma (scalar / pow2 4 <= (getOrder #c) / pow2 4)
-
-let lemma_test_2 #c scalar i = 
-  let o = getOrder #c in 
-  assert(scalar <= o - 1);
-  Math.Lemmas.lemma_div_le scalar (o - 1) (pow2 4);
-  assert(scalar / (pow2 4) <= (o - 1) / (pow2 4));
-  assert(o - 1 < o);
-  Math.Lemmas.lemma_div_le (o - 1) o (pow2 4);
-  assert((o - 1) / pow2 4 <= o / pow2 4);
-  assert(scalar / pow2 4 <= o / pow2 4)
-
-val lemma_test_1: #c: curve ->  scalar: nat {scalar < getOrder #c} 
-  -> i: nat {i > 0 /\ i < v ((size 2 *! getScalarLenBytes c))} -> 
-  Lemma (scalar / pow2 ((v (getScalarLen c) - i * 4)) <= (getOrder #c) / pow2 4)
-
-let lemma_test_1 #c scalar i = 
-  lemma_test_2 #c scalar i;
-  assert(v (getScalarLen c) - 4 * i >= 4);
-  Math.Lemmas.pow2_le_compat (v (getScalarLen c) - 4 * i) 4;
-  assert(pow2 (v (getScalarLen c) - 4 * i) >= pow2 4);
-  assert(1 / (pow2 (v (getScalarLen c) - 4 * i)) <= 1 / pow2 4);
-  Math.Lemmas.lemma_mult_le_left scalar (1 / (pow2 (v (getScalarLen c) - 4 * i))) (1 / pow2 4);
-  assert(scalar * (1 / (pow2 (v (getScalarLen c) - 4 * i))) <= scalar / pow2 4)
-
-
-let montgomery_ladder_2_precomputed #c #a p scalar tempBuffer =  
+let secret_to_public_radix #c #a p scalar tempBuffer =  
   let h0 = ST.get() in 
   radix_precomputed_upload_point p scalar;
   let h1 = ST.get() in 
@@ -422,7 +424,7 @@ let montgomery_ladder_2_precomputed #c #a p scalar tempBuffer =
   for (size 1) (size 2 *! getScalarLenBytes c) inv 
     (fun i -> 
       let h0_ = ST.get() in
-	lemma_test_1 #c (scalar_as_nat (as_seq h0 scalar)) (v i);
+	lemma_scalar_less_than_order #c (scalar_as_nat (as_seq h0 scalar)) (v i);
       radix_step_precomputed p tempBuffer scalar i;
 	Spec.ECC.Radix.pred0 #c #Affine (fromDomainPoint #c #DH (point_as_nat c h0_ p)) (as_seq h0_ scalar) (basePoint #c) (v i - 1))
 
@@ -440,6 +442,15 @@ let tableInvariant (c: curve) (h: mem) (precomputedTable: lbuffer uint64 (getPoi
     ~ (isPointAtInfinity #c p1) /\ pointEqual pi (point_mult #c i p1))
 
 
+val getPointTableLemma: #c: curve 
+  -> table: lbuffer uint64 (getPointLenU64 c *! 16ul) 
+  -> i: size_t {v i < 16} -> 
+  Lemma (getPointTable c table (v i) == gsub table (i *! getPointLenU64 c) (getPointLenU64 c))
+
+let getPointTableLemma #c table i = 
+  assert(getPointTable c table (v i) == gsub table (i *! getPointLenU64 c) (getPointLenU64 c))
+
+
 val getPointPrecomputedTable_: #c: curve -> k: size_t {v k < 16}
   -> precomputedTable: lbuffer uint64 (getPointLenU64 c *! 16ul)
   -> bits: uint64
@@ -447,33 +458,34 @@ val getPointPrecomputedTable_: #c: curve -> k: size_t {v k < 16}
   Stack unit 
   (requires fun h -> live h precomputedTable /\ live h r /\ disjoint r precomputedTable /\
     point_eval c h r /\ (
-    forall (i: nat {i < 16}). let pi = getPointTable c precomputedTable i in point_eval c h pi) /\ (
     forall (i: nat {i < 16}). 
-      let pi = fromDomainPoint #c #DH (point_as_nat c h (getPointTable c precomputedTable i)) in 
-      let p0 = fromDomainPoint #c #DH (point_as_nat c h (getPointTable c precomputedTable 1)) in 
-      pointEqual pi (point_mult #c i p0)))
+      let pi = getPointTable c precomputedTable i in
+      let p1 = getPointTable c precomputedTable 1 in 
+      point_eval c h pi /\ point_eval c h p1 /\ (
+      let pi = fromDomainPoint #c #DH (point_as_nat c h pi) in 
+      let p0 = fromDomainPoint #c #DH (point_as_nat c h p1) in 
+      pointEqual pi (point_mult #c i p0))))
   (ensures fun h0 _ h1 -> modifies (loc r) h0 h1 /\ point_eval c h1 r /\ (
-    let p0 = fromDomainPoint #c #DH (point_as_nat c h0 (getPointTable c precomputedTable 1)) in 
+    let p1 = getPointTable c precomputedTable 1 in 
+    let p1 = fromDomainPoint #c #DH (point_as_nat c h0 p1) in 
     let pi = fromDomainPoint #c #DH (point_as_nat c h1 r) in 
     if v bits = v k then 
-      pointEqual pi (point_mult #c (v k) p0)
+      pointEqual pi (point_mult #c (v k) p1)
     else 
       point_as_nat c h1 r == point_as_nat c h0 r))
 
 let getPointPrecomputedTable_ #c k precomputedTable bits r = 
-  let h0 = ST.get() in 
+  let h0 = ST.get() in
   let mask = eq_mask bits (to_u64 k) in 
     eq_mask_lemma bits (to_u64 k);
 
-  let pointLen = getPointLenU64 c *! k in 
+  let pointLen = k *! getPointLenU64 c in 
   let coordLen = getCoordinateLenU64 c in 
+  let lut_cmb = sub precomputedTable pointLen (getPointLenU64 c)  in 
 
-
-  let lut_cmb = sub precomputedTable pointLen (getPointLenU64 c) in 
-
-  let lut_cmb_x = sub precomputedTable pointLen coordLen in 
-  let lut_cmb_y = sub precomputedTable (pointLen +! coordLen) coordLen in
-  let lut_cmb_z = sub precomputedTable (pointLen +! size 2 *! coordLen) coordLen in 
+  let lut_cmb_x = sub lut_cmb (size 0) coordLen in 
+  let lut_cmb_y = sub lut_cmb coordLen coordLen in
+  let lut_cmb_z = sub lut_cmb (size 2 *! coordLen) coordLen in 
 
   let rX = sub r (size 0) coordLen in 
   let rY = sub r coordLen coordLen in 
@@ -481,17 +493,22 @@ let getPointPrecomputedTable_ #c k precomputedTable bits r =
 
   let h1 = ST.get() in 
   
-  copy_conditional #c rX lut_cmb_x mask;
+  copy_conditional #c rX lut_cmb_x mask; 
   copy_conditional #c rY lut_cmb_y mask;
-  copy_conditional #c rZ lut_cmb_z mask
+  copy_conditional #c rZ lut_cmb_z mask;
 
+  let h2 = ST.get() in 
 
+  getPointTableLemma precomputedTable k;
 
+  let p1 = getPointTable c precomputedTable 1 in 
+  let p1 = fromDomainPoint #c #DH (point_as_nat c h0 p1) in 
 
-val getPointTableLemma: #c: curve -> table: lbuffer uint64 (getPointLenU64 c *! 16ul) -> i: size_t {v i < 16} -> Lemma 
-  (getPointTable c table (v i) == gsub table (getPointLenU64 c *! i) (getPointLenU64 c))
-
-let getPointTableLemma #c table i = ()
+  assert(if v mask = 0 
+    then 
+      point_as_nat c h2 r == point_as_nat c h1 r
+    else 
+      pointEqual #c (fromDomainPoint #c #DH (point_as_nat c h2 r)) (fromDomainPoint #c #DH (point_as_nat c h1 lut_cmb)))
 
 
 val getPointTableLemma_1: #c: curve -> table: lbuffer uint64 (getPointLenU64 c *! 16ul) -> Lemma
@@ -500,36 +517,51 @@ val getPointTableLemma_1: #c: curve -> table: lbuffer uint64 (getPointLenU64 c *
 let getPointTableLemma_1 #c table = ()
 
 
-val lemma_test3__: #c: curve -> p: point c -> modified: LowStar.Monotonic.Buffer.loc -> h0: mem 
+val lemma_preserves_precomputed_table0: #c: curve 
+  -> p: point c 
+  -> modified: LowStar.Monotonic.Buffer.loc 
+  -> h0: mem 
   -> h1: mem {live h0 p /\ modifies modified h0 h1 /\ LowStar.Buffer.loc_disjoint (loc p) modified /\ point_eval c h0 p} -> 
-  Lemma (
-    point_eval c h1 p /\ point_as_nat c h0 p == point_as_nat c h1 p /\ 
+  Lemma (point_eval c h1 p /\ point_as_nat c h0 p == point_as_nat c h1 p /\ 
     fromDomainPoint #c #DH (point_as_nat c h0 p) == fromDomainPoint #c #DH (point_as_nat c h1 p))
 
-let lemma_test3__ #c p r h0 h1 = 
+let lemma_preserves_precomputed_table0 #c p r h0 h1 = 
   assert(as_nat c h0 (gsub p (size 0) (getCoordinateLenU64 c)) == as_nat c h1 (gsub p (size 0) (getCoordinateLenU64 c)));
   assert(as_nat c h0 (gsub p (getCoordinateLenU64 c) (getCoordinateLenU64 c)) == as_nat c h1 (gsub p (getCoordinateLenU64 c) (getCoordinateLenU64 c)));
   assert(as_nat c h0 (gsub p (2ul *! getCoordinateLenU64 c) (getCoordinateLenU64 c)) == as_nat c h1 (gsub p (2ul *! getCoordinateLenU64 c) (getCoordinateLenU64 c)))
 
 
-val lemma_test3_0: #c: curve -> precomputedTable: lbuffer uint64 (getPointLenU64 c *! 16ul) 
-  -> h0: mem -> h1: mem -> i: nat {i < 16} -> modified: LowStar.Monotonic.Buffer.loc -> Lemma
+val lemma_preserves_precomputed_table1: #c: curve 
+  -> precomputedTable: lbuffer uint64 (getPointLenU64 c *! 16ul) 
+  -> h0: mem 
+  -> h1: mem 
+  -> i: nat {i < 16} 
+  -> modified: LowStar.Monotonic.Buffer.loc -> 
+  Lemma
   (requires (live h0 precomputedTable /\ LowStar.Buffer.loc_disjoint modified (loc precomputedTable) /\ 
     modifies modified h0 h1 /\ (
     let pi = getPointTable c precomputedTable i in point_eval c h0 pi)))
   (ensures (
-   let pi = getPointTable c precomputedTable i in 
-   point_eval c h1 pi /\ point_as_nat c h0 pi == point_as_nat c h1 pi /\
-   fromDomainPoint #c #DH (point_as_nat c h0 pi) == fromDomainPoint #c #DH (point_as_nat c h1 pi)))
+    let pi = getPointTable c precomputedTable i in 
+    point_eval c h1 pi /\ point_as_nat c h0 pi == point_as_nat c h1 pi /\
+    fromDomainPoint #c #DH (point_as_nat c h0 pi) == fromDomainPoint #c #DH (point_as_nat c h1 pi)))
 
-let lemma_test3_0 #c precomputedTable h0 h1 i modified = 
+let lemma_preserves_precomputed_table1 #c precomputedTable h0 h1 i modified = 
   let p = getPointTable c precomputedTable i in 
   getPointTableLemma #c precomputedTable (size i);
-  lemma_test3__ #c p modified h0 h1
+  assert (p == gsub precomputedTable (size i *! getPointLenU64 c) (getPointLenU64 c));
+  assert (LowStar.Buffer.loc_disjoint modified (loc precomputedTable));
+  assert (LowStar.Buffer.loc_disjoint modified (loc p));
+  lemma_preserves_precomputed_table0 #c p modified h0 h1
 
 
-val lemma_test3_1: #c: curve -> precomputedTable: lbuffer uint64 (getPointLenU64 c *! 16ul) 
-  -> h0: mem -> h1: mem -> modified: LowStar.Monotonic.Buffer.loc -> i: nat {i < 16} -> Lemma
+val lemma_preserves_precomputed_table2: #c: curve 
+  -> precomputedTable: lbuffer uint64 (getPointLenU64 c *! 16ul) 
+  -> h0: mem 
+  -> h1: mem 
+  -> modified: LowStar.Monotonic.Buffer.loc 
+  -> i: nat {i < 16} -> 
+  Lemma
   (requires (live h0 precomputedTable /\ modifies modified h0 h1 /\ 
     LowStar.Buffer.loc_disjoint modified (loc precomputedTable) /\ (
     let pi = getPointTable c precomputedTable i in
@@ -542,15 +574,19 @@ val lemma_test3_1: #c: curve -> precomputedTable: lbuffer uint64 (getPointLenU64
     point_eval c h1 pi /\ point_eval c h1 p0 /\ 
     pointEqual (fromDomainPoint #c #DH (point_as_nat c h1 pi)) (point_mult #c i (fromDomainPoint #c #DH (point_as_nat c h1 p0)))))
 
-let lemma_test3_1 #c precomputedTable h0 h1 r i = 
-  lemma_test3_0 #c precomputedTable h0 h1 i r;
-  lemma_test3_0 #c precomputedTable h0 h1 1 r
+let lemma_preserves_precomputed_table2 #c precomputedTable h0 h1 r i = 
+  lemma_preserves_precomputed_table1 #c precomputedTable h0 h1 i r;
+  lemma_preserves_precomputed_table1 #c precomputedTable h0 h1 1 r
 
 
-val lemma_test3: #c: curve -> precomputedTable: lbuffer uint64 (getPointLenU64 c *! 16ul) 
-  -> h0: mem -> h1: mem -> modified: LowStar.Monotonic.Buffer.loc -> Lemma
-  (requires (live h0 precomputedTable /\ 
-    LowStar.Buffer.loc_disjoint modified (loc precomputedTable) /\ modifies modified h0 h1 /\ (
+val lemma_preserves_precomputed_table_: #c: curve 
+  -> precomputedTable: lbuffer uint64 (getPointLenU64 c *! 16ul) 
+  -> h0: mem 
+  -> h1: mem 
+  -> modified: LowStar.Monotonic.Buffer.loc -> 
+  Lemma
+  (requires (live h0 precomputedTable /\ LowStar.Buffer.loc_disjoint modified (loc precomputedTable) /\ 
+    modifies modified h0 h1 /\ (
     forall (i: nat {i < 16}). ( 
       let pi = getPointTable c precomputedTable i in 
       let p1 = getPointTable c precomputedTable 1 in
@@ -566,15 +602,15 @@ val lemma_test3: #c: curve -> precomputedTable: lbuffer uint64 (getPointLenU64 c
       let p0 = fromDomainPoint #c #DH (point_as_nat c h1 (getPointTable c precomputedTable 1)) in 
       pointEqual pi (point_mult #c i p0))))
 
-let lemma_test3 #c precomputedTable h0 h1 r = 
+let lemma_preserves_precomputed_table_ #c precomputedTable h0 h1 r = 
   let a : Type = (a: nat {a < 16}) in 
-  let p : (a -> GTot Type)  = 
+  let p : (a -> GTot Type) = 
     fun i -> 
       let pi = getPointTable c precomputedTable i in 
       let p1 = getPointTable c precomputedTable 1 in 
       point_eval c h1 pi /\ point_eval c h1 p1 /\ 
       pointEqual (fromDomainPoint #c #DH (point_as_nat c h1 pi)) (point_mult #c i (fromDomainPoint #c #DH (point_as_nat c h1 p1))) in 
-  let pred: (x : a -> Lemma (p x)) = lemma_test3_1 #c precomputedTable h0 h1 r in 
+  let pred: (x : a -> Lemma (p x)) = lemma_preserves_precomputed_table2 #c precomputedTable h0 h1 r in 
   Classical.forall_intro #a #_ pred
 
 
@@ -611,15 +647,13 @@ let getPointPrecomputedTable_1 #c precomputedTable bits r =
 	(fromDomainPoint #c #DH (point_as_nat c h0 p0)))
     else
       point_as_nat c h r == point_as_nat c h0 r)) in 
-
   let f = fun (k: size_t {0 <= v k /\ v k < 16})  ->
     let h0_ = ST.get() in 
     getPointPrecomputedTable_ k precomputedTable bits r; 
     let h1 = ST.get() in
-    lemma_test3 #c precomputedTable h0 h1 (loc r);
+    lemma_preserves_precomputed_table_ #c precomputedTable h0 h1 (loc r);
     assert (modifies (loc r) h0 h0_);
-    lemma_test3__ (getPointTable c precomputedTable 1) (loc r) h0 h0_ in 
-
+    lemma_preserves_precomputed_table0 (getPointTable c precomputedTable 1) (loc r) h0 h0_ in 
   Lib.Loops.for (size 0) (size 16) inv f
 
 
@@ -645,17 +679,15 @@ val getPointPrecomputedTable: #c: curve -> #buf_type: buftype
 
 
 let getPointPrecomputedTable #c #buf_type scalar precomputedTable i pointToAdd = 
-  let h0 = ST.get() in 
+    let h0 = ST.get() in 
   let bits = getScalar_4_byBit #c scalar i in 
-  let h1 = ST.get() in 
-
+    let h1 = ST.get() in 
     Hacl.Impl.P.PointAdd.Aux.lemma_coord_eval c h0 h1 pointToAdd; 
-    lemma_test3 #c precomputedTable h0 h1 (loc pointToAdd); 
-  getPointPrecomputedTable_1 precomputedTable bits pointToAdd;  
-    lemma_test3__ (getPointTable c precomputedTable 1) pointToAdd h0 h1
+    lemma_preserves_precomputed_table_ #c precomputedTable h0 h1 (loc pointToAdd);
+  getPointPrecomputedTable_1 precomputedTable bits pointToAdd;
+    lemma_preserves_precomputed_table0 (getPointTable c precomputedTable 1) (loc pointToAdd) h0 h1
 
  
-
 inline_for_extraction noextract
 val montgomery_ladder_step_radix_0: #c: curve -> #buf_type: buftype
   -> p: point c 
@@ -680,7 +712,6 @@ val montgomery_ladder_step_radix_0: #c: curve -> #buf_type: buftype
     let bits = Math.Lib.arithmetic_shift_right (scalar_as_nat #c (as_seq h0 scalar)) (v (getScalarLen c) - (v i + 1) * 4) % pow2 4 in 
     pointEqual (fromDomainPoint #c #DH (point_as_nat c h1 r)) (Spec.ECC.Radix.getPrecomputedPoint #c #Jacobian p1 bits) /\   
     fromDomainPoint #c #DH (point_as_nat c h1 p) == Spec.ECC.Radix.getPointDoubleNTimes #c (fromDomainPoint #c #DH (point_as_nat c h0 p)) 4))
-
 
 let montgomery_ladder_step_radix_0 #c #b p scalar precomputedTable i tempBuffer r = 
     let h0 = ST.get() in 
@@ -712,13 +743,12 @@ let montgomery_ladder_step_radix_1_lemma #c k p0 p pi r i =
   let l = v (getScalarLen c) in 
   let si = Math.Lib.arithmetic_shift_right scalar (l - ((i - 1) + 2) * 4) % pow2 4 in 
   let pointRadixed = Spec.ECC.Radix.getPointDoubleNTimes #c p 4 in 
-  let pointPrecomputed = (Spec.ECC.Radix.getPrecomputedPoint #c #Jacobian p0 si) in 
+  let pointPrecomputed = Spec.ECC.Radix.getPrecomputedPoint #c #Jacobian p0 si in 
 
   not_equal_precomputed2 #c p0 p si;
   curve_order_is_the_smallest #c p0;
   curve_compatibility_with_translation_lemma pi pointPrecomputed pointRadixed; 
   curve_commutativity_lemma pointPrecomputed pointRadixed
-
 
 
 inline_for_extraction noextract
@@ -743,7 +773,6 @@ val montgomery_ladder_step_radix: #c: curve -> #buf_type: buftype
     let p = (fromDomainPoint #c #DH (point_as_nat c h0 p)) in 
     pointEqual #c r (Spec.ECC.Radix.radix_step #c #Jacobian (as_seq h0 scalar) p1 (v i - 1) p)))
 
-
 let montgomery_ladder_step_radix #c #b p scalar table i tempBuffer r = 
   let h0 = ST.get() in 
   montgomery_ladder_step_radix_0 p scalar table i tempBuffer r;
@@ -753,9 +782,9 @@ let montgomery_ladder_step_radix #c #b p scalar table i tempBuffer r =
   Hacl.Impl.P.PointAdd.Aux.lemma_coord_eval c h1 h2 r;
   
   let p1 = fromDomainPoint #c #DH (point_as_nat c h0 (getPointTable c table 1)) in 
-  let pi = (fromDomainPoint #c #DH (point_as_nat c h1 r)) in 
+  let pi = fromDomainPoint #c #DH (point_as_nat c h1 r) in 
   let r =  fromDomainPoint #c #DH (point_as_nat c h2 p) in 
-  let p = (fromDomainPoint #c #DH (point_as_nat c h0 p)) in 
+  let p =  fromDomainPoint #c #DH (point_as_nat c h0 p) in 
 
   montgomery_ladder_step_radix_1_lemma #c (as_seq h0 scalar) p1 p pi r (v i)
 
@@ -767,8 +796,12 @@ let lemma_pointAtInfInDomain1 #c p =
   let (x, y, z) = p in 
   lemma_pointAtInfInDomain #c x y z
 
-val lemma_modifies_not_first_element_of_precomputed_table: #c: curve -> modified: LowStar.Monotonic.Buffer.loc 
-  -> h0: mem -> h1: mem -> table: lbuffer uint64 (getPointLenU64 c *! 16ul) -> 
+
+val lemma_modifies_not_first_element_of_precomputed_table: #c: curve 
+  -> modified: LowStar.Monotonic.Buffer.loc 
+  -> h0: mem 
+  -> h1: mem 
+  -> table: lbuffer uint64 (getPointLenU64 c *! 16ul) -> 
   Lemma 
   (requires (modifies modified h0 h1 /\ LowStar.Buffer.loc_disjoint modified (loc table) /\ live h0 table /\
     point_eval c h0 (getPointTable c table 1)))
@@ -780,14 +813,15 @@ val lemma_modifies_not_first_element_of_precomputed_table: #c: curve -> modified
 let lemma_modifies_not_first_element_of_precomputed_table #c modified h0 h1 table = 
   let p1 = getPointTable c table 1 in 
   getPointTableLemma_1 table;
-
+  
   assert(as_nat c h0 (gsub p1 (size 0) (getCoordinateLenU64 c)) == as_nat c h1 (gsub p1 (size 0) (getCoordinateLenU64 c)));
   assert(as_nat c h0 (gsub p1 (getCoordinateLenU64 c) (getCoordinateLenU64 c)) == as_nat c h1 (gsub p1 (getCoordinateLenU64 c) (getCoordinateLenU64 c)));
   assert(as_nat c h0 (gsub p1 (2ul *! getCoordinateLenU64 c) (getCoordinateLenU64 c)) == as_nat c h1 (gsub p1 (2ul *! getCoordinateLenU64 c) (getCoordinateLenU64 c)))
 
 
 inline_for_extraction noextract
-val generatePrecomputedTable_0: #c: curve -> precomputedTable: lbuffer uint64 (getPointLenU64 c *! 16ul) 
+val generatePrecomputedTable_0: #c: curve 
+  -> precomputedTable: lbuffer uint64 (getPointLenU64 c *! 16ul) 
   -> publicKey: point c -> 
   Stack unit
   (requires fun h -> live h precomputedTable /\ live h publicKey /\ point_eval c h publicKey /\ 
@@ -818,8 +852,8 @@ let generatePrecomputedTable_0 #c table publicKey =
   getPointTableLemma table (size 0);
   getPointTableLemma_1 table;
 
-  assert (getPointTable c table 0 == gsub table (pointLen *! size 0) pointLen);
-  assert (getPointTable c table 1 == gsub table (pointLen *! size 1) pointLen);
+  assert (getPointTable c table 0 == gsub table (size 0 *! pointLen) pointLen);
+  assert (getPointTable c table 1 == gsub table (size 1 *! pointLen) pointLen);
 
   let p1 = fromDomainPoint #c #DH (point_as_nat c h2 (getPointTable c table 1)) in 
   let p  = fromDomainPoint #c #DH (point_as_nat c h0 publicKey) in
@@ -829,10 +863,12 @@ let generatePrecomputedTable_0 #c table publicKey =
   point_mult_1 #c p1
 
 
-val lemma_disjoint_and_eval_points_upload_table: #c: curve -> i: size_t {v i >= 1 /\ v i <= 7} -> h: mem
+val lemma_disjoint_and_eval_points_upload_table: #c: curve
+  -> i: size_t {v i >= 1 /\ v i <= 7} 
+  -> h: mem
   -> table: lbuffer uint64 (getPointLenU64 c *! 16ul) -> 
   Lemma
-  (requires (forall (j: nat {j < 2 * v i}). let pi = getPointTable c table j in point_eval c h pi))
+  (requires (live h table /\ (forall (j: nat {j < 2 * v i}). let pi = getPointTable c table j in point_eval c h pi)))
   (ensures (
     let point1 = getPointTable c table 1 in 
     let point_n = getPointTable c table (v i) in 
@@ -850,19 +886,20 @@ let lemma_disjoint_and_eval_points_upload_table #c i h table =
     
   getPointTableLemma #c table i;
   getPointTableLemma_1 #c table;
+  assert (disjoint point_n point_2n)
 
-  assert(disjoint point_n point_2n /\ point_eval c h point_n /\ point_eval c h point1)
 
-
-val lemma_disjoint_and_eval_points_upload_table1: #c: curve -> i: size_t {v i >= 1 /\ v i <= 7} -> h0: mem -> h1: mem 
+val lemma_disjoint_and_eval_points_upload_table1: #c: curve 
+  -> i: size_t {v i >= 1 /\ v i <= 7} 
+  -> h0: mem 
+  -> h1: mem 
   -> table: lbuffer uint64 (getPointLenU64 c *! 16ul) 
   -> tempBuffer: lbuffer uint64 (size 17 *! getCoordinateLenU64 c) ->
   Lemma
   (requires (
     let point_2n = getPointTable c table (2 * v i) in 
     modifies (loc point_2n |+| loc tempBuffer) h0 h1 /\ disjoint table tempBuffer /\ live h0 table /\ (
-    forall (j: nat {j < 2 * v i}). 
-      let pi = getPointTable c table j in point_eval c h0 pi)))
+    forall (j: nat {j < 2 * v i}). let pi = getPointTable c table j in point_eval c h0 pi)))
   (ensures (
     let point1 = getPointTable c table 1 in 
     let point_n = getPointTable c table (v i) in 
@@ -873,7 +910,7 @@ val lemma_disjoint_and_eval_points_upload_table1: #c: curve -> i: size_t {v i >=
     point_as_nat c h0 point1 == point_as_nat c h1 point1))
 
 let lemma_disjoint_and_eval_points_upload_table1 #c i h0 h1 table tempBuffer = 
-  let pointLen = getPointLenU64 c in 
+  let pointLen = getPointLenU64 c in
   
   let point1 = gsub table pointLen pointLen in 
   let point_n = gsub table (i *! pointLen) pointLen in 
@@ -885,24 +922,44 @@ let lemma_disjoint_and_eval_points_upload_table1 #c i h0 h1 table tempBuffer =
   Hacl.Impl.P.PointAdd.Aux.lemma_coord_eval c h0 h1 point1
 
 
-val lemma_not_modifies_all_points_before_index: #c: curve -> i: size_t {v i >= 1 /\ v i <= 7} -> h0: mem -> h1: mem 
+val lemma_not_modifies_all_points_before_index: #c: curve 
+  -> i: size_t {v i >= 1 /\ v i <= 7} 
+  -> h0: mem 
+  -> h1: mem 
   -> table: lbuffer uint64 (getPointLenU64 c *! 16ul) 
-  -> tempBuffer: lbuffer uint64 (size 17 *! getCoordinateLenU64 c) ->
+  -> tempBuffer: LowStar.Monotonic.Buffer.loc ->
   Lemma 
-  (requires (live h0 table /\ live h0 tempBuffer /\ disjoint table tempBuffer /\ ( 
+  (requires (live h0 table /\ LowStar.Buffer.loc_disjoint (loc table) tempBuffer /\ ( 
     let point_2n = getPointTable c table (2 * v i) in 
     let point_2n_1 = getPointTable c table (2 * v i + 1) in 
-    modifies (loc point_2n |+| loc point_2n_1 |+| loc tempBuffer) h0 h1)))
+    modifies (loc point_2n |+| loc point_2n_1 |+| tempBuffer) h0 h1)))
   (ensures (
     let pointLen = getPointLenU64 c in 
     let allPointsBefore = gsub table (size 0) (2ul *! i *! pointLen) in 
     as_seq h0 allPointsBefore == as_seq h1 allPointsBefore))
 
-let lemma_not_modifies_all_points_before_index #c i h0 h1 table tempBuffer = ()
+let lemma_not_modifies_all_points_before_index #c i h0 h1 table tempBuffer =
+  let pointLen = getPointLenU64 c in 
+  let allPointsBefore = gsub table (size 0) (2ul *! i *! pointLen) in 
+
+  let point_2n = getPointTable c table (2 * v i) in 
+  let point_2n_1 = getPointTable c table (2 * v i + 1) in 
+
+  getPointTableLemma table (size (2 * v i)); 
+  getPointTableLemma table (size (2 * v i + 1)); 
+
+  assert(point_2n == gsub table (size (2 * v i) *! getPointLenU64 c) (getPointLenU64 c));
+  assert(point_2n_1 == gsub table (size (2 * v i + 1) *! getPointLenU64 c) (getPointLenU64 c));
+
+  assert(as_seq h0 allPointsBefore == as_seq h1 allPointsBefore)
 
 
-val lemma_not_modifies_point_k: #c: curve -> i: size_t {v i >= 1 /\ v i <= 7} -> h0: mem -> h1: mem 
-  -> table: lbuffer uint64 (getPointLenU64 c *! 16ul) -> k: nat {k < 2 * v i} ->
+val lemma_not_modifies_point_k: #c: curve 
+  -> i: size_t {v i >= 1 /\ v i <= 7} 
+  -> h0: mem 
+  -> h1: mem 
+  -> table: lbuffer uint64 (getPointLenU64 c *! 16ul) 
+  -> k: nat {k < 2 * v i} ->
   Lemma 
   (requires (
     let pointLen = getPointLenU64 c in 
@@ -962,7 +1019,10 @@ let lemma_point_eval_if_point_did_not_change_ #c i h0 h1 table j =
   lemma_getZ #c (getPointTable c table j)
 
 
-val lemma_point_eval_if_point_did_not_change: #c: curve -> i: size_t {v i >= 1 /\ v i <= 7} -> h0: mem -> h1: mem 
+val lemma_point_eval_if_point_did_not_change: #c: curve 
+  -> i: size_t {v i >= 1 /\ v i <= 7} 
+  -> h0: mem 
+  -> h1: mem 
   -> table: lbuffer uint64 (getPointLenU64 c *! 16ul) ->
   Lemma (requires (live h0 table /\ (
     let pointLen = getPointLenU64 c in 
@@ -1013,7 +1073,7 @@ val lemma_preserves_precomputed_table: #c: curve -> i: size_t {v i >= 1 /\ v i <
       pointEqual (fromDomainPoint #c #DH (point_as_nat c h1 point_2n)) (point_mult #c (2 * v i) p1) /\ 
       pointEqual (fromDomainPoint #c #DH (point_as_nat c h1 point_2n_1)) (point_mult #c (2 * v i + 1) p1))))))
   (ensures (
-      forall (j: nat {j <= 2 * v i + 1}). 
+    forall (j: nat {j <= 2 * v i + 1}). 
       let p1 = getPointTable c table 1 in 
       let pi = getPointTable c table j in point_eval c h1 pi /\ point_eval c h1 p1 /\ 
       point_as_nat c h0 p1 == point_as_nat c h1 p1 /\ (
@@ -1022,7 +1082,7 @@ val lemma_preserves_precomputed_table: #c: curve -> i: size_t {v i >= 1 /\ v i <
       ~ (isPointAtInfinity #c p1) /\ (pointEqual pi (point_mult #c j p1)))))
 
 let lemma_preserves_precomputed_table #c i h0 h1 table tempBuffer = 
-  lemma_not_modifies_all_points_before_index i h0 h1 table tempBuffer;
+  lemma_not_modifies_all_points_before_index i h0 h1 table (loc tempBuffer);
   lemma_point_eval_if_point_did_not_change #c i h0 h1 table;
   lemma_not_modifies_point_k i h0 h1 table 1
 
@@ -1089,7 +1149,6 @@ let lemma_two_points_different_coeff_not_equal #c p0 pk p qk q =
       curve_compatibility_with_translation_lemma #c p q (inverseP);
       assert(False)
     end
-
 
 
 val generatePrecomputedResultOfPointAddAndDouble: #c: curve 
@@ -1173,7 +1232,6 @@ let generatePrecomputedTable_step #c table i tempBuffer =
   generatePrecomputedResultOfPointAddAndDouble #c table (v i) h0 h1 h2;
   lemma_preserves_precomputed_table i h0 h2 table tempBuffer
 
-  
 
 val generatePrecomputedTable_loop: #c: curve -> precomputedTable: lbuffer uint64 (getPointLenU64 c *! 16ul) 
   -> tempBuffer: lbuffer uint64 (size 17 *! getCoordinateLenU64 c) ->
@@ -1203,7 +1261,8 @@ let generatePrecomputedTable_loop #c table tempBuffer =
 
 
 [@ CInline]
-val generatePrecomputedTable: #c: curve -> precomputedTable: lbuffer uint64 (getPointLenU64 c *! 16ul) 
+val generatePrecomputedTable: #c: curve 
+  -> precomputedTable: lbuffer uint64 (getPointLenU64 c *! 16ul) 
   -> publicKey: point c 
   -> tempBuffer: lbuffer uint64 (size 17 *! getCoordinateLenU64 c) -> Stack unit  
   (requires fun h -> 
@@ -1223,7 +1282,10 @@ let generatePrecomputedTable #c table publicKey tempBuffer =
   generatePrecomputedTable_loop #c table tempBuffer
 
 
-val lemma_modifies_not_tb_invariant_holds: #c: curve -> modified: LowStar.Monotonic.Buffer.loc -> h0: mem -> h1: mem 
+val lemma_modifies_not_tb_invariant_holds: #c: curve 
+  -> modified: LowStar.Monotonic.Buffer.loc
+  -> h0: mem 
+  -> h1: mem 
   -> table: lbuffer uint64 (getPointLenU64 c *! 16ul) -> 
   Lemma 
   (requires (tableInvariant c h0 table /\ modifies modified h0 h1 /\ 
@@ -1231,12 +1293,12 @@ val lemma_modifies_not_tb_invariant_holds: #c: curve -> modified: LowStar.Monoto
   (ensures (tableInvariant c h1 table))
 
 let lemma_modifies_not_tb_invariant_holds #c modified h0 h1 table = 
-  lemma_test3 #c table h0 h1 modified;
+  lemma_preserves_precomputed_table_ #c table h0 h1 modified;
   lemma_modifies_not_first_element_of_precomputed_table modified h0 h1 table
 
 
 inline_for_extraction noextract
-val montgomery_ladder_2_: #c: curve -> #buf_type: buftype 
+val scalar_mult_radix__: #c: curve -> #buf_type: buftype 
   -> p: point c
   -> scalar: scalar_t #buf_type #c 
   -> tempBuffer: lbuffer uint64 (size 17 *! getCoordinateLenU64 c) 
@@ -1259,8 +1321,7 @@ val montgomery_ladder_2_: #c: curve -> #buf_type: buftype
     let p_n = fromDomainPoint #c #DH (point_as_nat c h1 p) in 
     pointEqual p_n (point_mult #c (scalar_as_nat (as_seq h0 scalar)) p1)))
 
-
-let montgomery_ladder_2_ #c p scalar tempBuffer r precomputedTable =  
+let scalar_mult_radix__ #c p scalar tempBuffer r precomputedTable =  
   let h0 = ST.get() in 
   let inv h (i: nat {i <= 2 * v (getScalarLenBytes c)}) =
     live h precomputedTable /\ live h r /\ live h tempBuffer /\ live h scalar /\ live h p /\
@@ -1279,7 +1340,7 @@ let montgomery_ladder_2_ #c p scalar tempBuffer r precomputedTable =
   (fun j -> 
     let h0_ = ST.get() in
     
-    lemma_test_1 #c (scalar_as_nat (as_seq h0 scalar)) (v j);
+    lemma_scalar_less_than_order #c (scalar_as_nat (as_seq h0 scalar)) (v j);
     montgomery_ladder_step_radix #c p scalar precomputedTable j tempBuffer r;
     let h1_ = ST.get() in 
    
@@ -1300,7 +1361,7 @@ let montgomery_ladder_2_ #c p scalar tempBuffer r precomputedTable =
 
 
 inline_for_extraction noextract
-val montgomery_ladder_2: #c: curve -> #buf_type: buftype 
+val scalar_mult_radix_: #c: curve -> #buf_type: buftype 
   -> p: point c
   -> scalar: scalar_t #buf_type #c 
   -> tempBuffer: lbuffer uint64 (size 17 *! getCoordinateLenU64 c) 
@@ -1318,7 +1379,7 @@ val montgomery_ladder_2: #c: curve -> #buf_type: buftype
     let p_n = fromDomainPoint #c #DH (point_as_nat c h1 p) in 
     pointEqual p_n (point_mult #c (scalar_as_nat (as_seq h0 scalar)) p1)))
 
-let montgomery_ladder_2 #c p scalar tempBuffer r precomputedTable = 
+let scalar_mult_radix_ #c p scalar tempBuffer r precomputedTable = 
   let h0 = ST.get() in 
   getPointPrecomputedTable #c scalar precomputedTable (size 0) p;
 
@@ -1331,8 +1392,7 @@ let montgomery_ladder_2 #c p scalar tempBuffer r precomputedTable =
   Math.Lemmas.small_mod (scalar_as_nat (as_seq h0 scalar) / pow2 (v (getScalarLen c) - 4)) (pow2 4);
 
   lemma_modifies_not_first_element_of_precomputed_table (loc p) h0 h1 precomputedTable;
-  montgomery_ladder_2_ p scalar tempBuffer r precomputedTable
-
+  scalar_mult_radix__ p scalar tempBuffer r precomputedTable
 
 
 (* the same as in DH *)
@@ -1347,26 +1407,11 @@ let lemma_zero_point_zero_coordinates c h p =
   Hacl.Impl.P.PointAdd.Aux.lemma_point_eval_if_zero c p h
 
 
-val lemma_point_mult_equal_points: #c: curve -> p0: Spec.ECC.point #c -> i: nat 
-  -> p1: Spec.ECC.point #c {pointEqual p0 p1} -> 
-  Lemma (pointEqual (point_mult i p0) (point_mult i p1))
-
-let rec lemma_point_mult_equal_points #c p0 i p1 = 
-  match i with 
-  |0 -> point_mult_0 p0 0; point_mult_0 p1 0
-  |_ -> 
-    lemma_point_mult_equal_points #c p0 (i - 1) p1;
-    point_mult_ext (i - 1) p0;
-    point_mult_ext (i - 1) p1; 
-    curve_compatibility_with_translation_lemma p0 p1 (point_mult (i - 1) p0);
-    curve_compatibility_with_translation_lemma_1  (point_mult (i - 1) p0) (point_mult (i - 1) p1) p1
-
-
 inline_for_extraction noextract
-val scalar_multiplication_t_0: #c: curve -> #t:buftype
+val scalar_mult_radix: #c: curve -> #t:buftype
   -> publicKey: point c 
   -> scalar: scalar_t #t #c 
-  -> tempBuffer: lbuffer uint64 (size 17 *! getCoordinateLenU64 c) ->
+  -> tempBuffer: lbuffer uint64 (size 20 *! getCoordinateLenU64 c) ->
   Stack unit 
   (requires fun h -> live h publicKey /\ live h scalar /\ live h tempBuffer /\
     LowStar.Monotonic.Buffer.all_disjoint [loc publicKey; loc tempBuffer; loc scalar] /\ 
@@ -1379,13 +1424,12 @@ val scalar_multiplication_t_0: #c: curve -> #t:buftype
     let p  = fromDomainPoint #c #DH (point_as_nat c h0 publicKey) in
     pointEqual result (point_mult #c (scalar_as_nat (as_seq h0 scalar)) p)))
 
-
-
-let scalar_multiplication_t_0 #c publicKey scalar tempBuffer = 
+let scalar_mult_radix #c publicKey scalar tempBuffer = 
   let h0 = ST.get() in 
   push_frame(); 
     let precomputedTable = create (size 16 *! getPointLenU64 c) (u64 0) in 
     let tempPoint = create (getPointLenU64 c) (u64 0) in 
+    let tempBuffer = sub tempBuffer (size 0) (size 17 *! getCoordinateLenU64 c) in 
   let h1 = ST.get() in 
   Hacl.Impl.P.PointAdd.Aux.lemma_coord_eval c h0 h1 publicKey;
   generatePrecomputedTable precomputedTable publicKey tempBuffer;
@@ -1398,37 +1442,12 @@ let scalar_multiplication_t_0 #c publicKey scalar tempBuffer =
   Hacl.Impl.P.PointAdd.Aux.lemma_coord_eval c h1 h2 tempPoint;
   Hacl.Impl.P.PointAdd.Aux.lemma_coord_eval c h1 h2 publicKey;
     
-  montgomery_ladder_2 publicKey scalar tempBuffer tempPoint precomputedTable;
-
+  scalar_mult_radix_ publicKey scalar tempBuffer tempPoint precomputedTable;
+  
   let h3 = ST.get() in 
 
-  lemma_point_mult_equal_points #c (fromDomainPoint #c #DH (point_as_nat c h1 publicKey)) (scalar_as_nat (as_seq h2 scalar)) (fromDomainPoint #c #DH (point_as_nat c h2 (getPointTable c precomputedTable 1))) ;
+  lemma_point_mult_equal_points #c (fromDomainPoint #c #DH (point_as_nat c h1 publicKey)) (fromDomainPoint #c #DH (point_as_nat c h2 (getPointTable c precomputedTable 1))) (scalar_as_nat (as_seq h2 scalar));
 
-  assert(
-    let result = fromDomainPoint #c #DH (point_as_nat c h3 publicKey) in 
-    let p  = fromDomainPoint #c #DH (point_as_nat c h0 publicKey) in
-    pointEqual result (point_mult #c (scalar_as_nat (as_seq h0 scalar)) p));
-  admit(); 
-  pop_frame()
-
-
-inline_for_extraction noextract
-val secretToPublic_0: #c: curve -> #t: buftype -> q: point c -> result: point c -> 
-  scalar: lbuffer_t t uint8 (getScalarLenBytes c) -> 
-  tempBuffer: lbuffer uint64 (size 17 *! getCoordinateLenU64 c) ->
-  Stack unit 
-  (requires fun h -> live h q /\ live h result /\ live h scalar /\ live h tempBuffer /\
-    LowStar.Monotonic.Buffer.all_disjoint [loc q; loc tempBuffer; loc scalar] /\
-    disjoint q result /\ disjoint result tempBuffer /\ disjoint result scalar)
-  (ensures fun h0 _ h1 -> modifies (loc q |+| loc result |+| loc tempBuffer) h0 h1 /\ point_eval c h1 q /\ (
-    let i1 = basePoint #c in 
-    point_mult_0 #c i1 0; 
-    let pD = fromDomainPoint #c #DH (point_as_nat c h1 q) in
-    let r0, _ = montgomery_ladder_spec_left (as_seq h0 scalar) (pointAtInfinity #c , i1) in pD == r0))
-
-
-let secretToPublic_0 #c q result scalar tempBuffer = 
-(*   uploadStartPointsS2P q result; 
-  montgomery_ladder q result scalar tempBuffer
- *)  montgomery_ladder_2_precomputed result scalar tempBuffer;
-  copy q result
+  pop_frame();
+  let h4 = ST.get() in 
+  Hacl.Impl.P.PointAdd.Aux.lemma_coord_eval c h3 h4 publicKey
